Makefile
@@ -1,0 +1,5 @@
+all:
+	rm -rf ./html/*
+	coqc systemf.v
+	coqdoc -utf8 -g --no-index -d html systemf.v
+	scp html/systemf.html sboul434@ssh.eleves.ens-rennes.fr:/home/sboul434/public_html/systemf/index.html
